<?xml version="1.0"?>
<rdf:RDF xmlns="https://w3id.org/polifonia/ontology/cometa/"
     xml:base="https://w3id.org/polifonia/ontology/cometa/"
     xmlns:dc="http://purl.org/dc/elements/1.1/"
     xmlns:l0="https://w3id.org/italia/onto/l0/"
     xmlns:mm="https://w3id.org/polifonia/ontology/music-meta/"
     xmlns:mx="https://w3id.org/polifonia/ontology/music-algorithm/"
     xmlns:ns="http://www.w3.org/2006/vcard/ns#"
     xmlns:owl="http://www.w3.org/2002/07/owl#"
     xmlns:rdf="http://www.w3.org/1999/02/22-rdf-syntax-ns#"
     xmlns:xml="http://www.w3.org/XML/1998/namespace"
     xmlns:xsd="http://www.w3.org/2001/XMLSchema#"
     xmlns:core="https://w3id.org/polifonia/ontology/core/"
     xmlns:dcat="http://www.w3.org/ns/dcat#"
     xmlns:foaf="http://xmlns.com/foaf/0.1/"
     xmlns:opla="http://www.ontologydesignpatterns.org/opla/"
     xmlns:prov="http://www.w3.org/ns/prov#"
     xmlns:rdfs="http://www.w3.org/2000/01/rdf-schema#"
     xmlns:opla1="http://ontologydesignpatterns.org/opla/"
     xmlns:terms="http://purl.org/dc/terms/">
    <owl:Ontology rdf:about="https://w3id.org/polifonia/ontology/cometa/">
        <owl:versionIRI rdf:resource="https://w3id.org/polifonia/ontology/cometa/1.0/"/>
        <owl:imports rdf:resource="https://w3id.org/polifonia/ontology/music-meta/1.0/"/>
        <dc:creator xml:lang="en">Andrea Poltronieri</dc:creator>
        <dc:creator xml:lang="en">Jacopo de Berardinis</dc:creator>
        <dc:creator>Nicolas Lazzari</dc:creator>
        <dc:license rdf:resource="https://creativecommons.org/licenses/by-sa/4.0/"/>
        <terms:license rdf:resource="https://creativecommons.org/licenses/by-sa/4.0/"/>
        <rdfs:comment xml:lang="en">An extension of Music Meta to describe the metadata of music collections, corpora, containers, or simply music datasets.</rdfs:comment>
        <rdfs:label xml:lang="en">CoMeta Ontology</rdfs:label>
        <owl:versionInfo xml:lang="en">1.0</owl:versionInfo>
    </owl:Ontology>
    


    <!-- 
    ///////////////////////////////////////////////////////////////////////////////////////
    //
    // Object Properties
    //
    ///////////////////////////////////////////////////////////////////////////////////////
     -->

    


    <!-- https://w3id.org/polifonia/ontology/cometa/annotatesData -->

    <owl:ObjectProperty rdf:about="https://w3id.org/polifonia/ontology/cometa/annotatesData">
        <rdfs:domain rdf:resource="https://w3id.org/polifonia/ontology/cometa/ContentAnnotation"/>
        <rdfs:range rdf:resource="https://w3id.org/polifonia/ontology/cometa/ContentDescriptor"/>
        <rdfs:range rdf:resource="https://w3id.org/polifonia/ontology/cometa/RawDataContent"/>
        <rdfs:comment xml:lang="en">Associates an annotation to the raw data, or data descriptor, it annotates</rdfs:comment>
        <rdfs:label xml:lang="en">annotates data</rdfs:label>
    </owl:ObjectProperty>
    


    <!-- https://w3id.org/polifonia/ontology/cometa/describesData -->

    <owl:ObjectProperty rdf:about="https://w3id.org/polifonia/ontology/cometa/describesData">
        <rdfs:domain rdf:resource="https://w3id.org/polifonia/ontology/cometa/ContentDescriptor"/>
        <rdfs:range rdf:resource="https://w3id.org/polifonia/ontology/cometa/RawDataContent"/>
        <rdfs:comment xml:lang="en">Associates a data descriptor (e.g. features, encodings) to the raw data they were derived from</rdfs:comment>
        <rdfs:label xml:lang="en">describes data</rdfs:label>
    </owl:ObjectProperty>
    


    <!-- https://w3id.org/polifonia/ontology/cometa/extends -->

    <owl:ObjectProperty rdf:about="https://w3id.org/polifonia/ontology/cometa/extends">
        <rdfs:domain rdf:resource="https://w3id.org/polifonia/ontology/cometa/ontology_URI#Dataset"/>
        <rdfs:range rdf:resource="https://w3id.org/polifonia/ontology/cometa/ontology_URI#Dataset"/>
        <rdfs:label xml:lang="en">extends</rdfs:label>
    </owl:ObjectProperty>
    


    <!-- https://w3id.org/polifonia/ontology/cometa/hasAPI -->

    <owl:ObjectProperty rdf:about="https://w3id.org/polifonia/ontology/cometa/hasAPI">
        <rdfs:domain rdf:resource="https://w3id.org/polifonia/ontology/cometa/ontology_URI#DataAvailability"/>
        <rdfs:range rdf:resource="https://w3id.org/polifonia/ontology/cometa/ontology_URI#API"/>
        <rdfs:comment xml:lang="en">Associates an API to the availability information of a dataset</rdfs:comment>
        <rdfs:label xml:lang="en">has API</rdfs:label>
    </owl:ObjectProperty>
    


    <!-- https://w3id.org/polifonia/ontology/cometa/hasAccessibility -->

    <owl:ObjectProperty rdf:about="https://w3id.org/polifonia/ontology/cometa/hasAccessibility">
        <rdfs:domain rdf:resource="https://w3id.org/polifonia/ontology/cometa/ontology_URI#DataAvailability"/>
        <rdfs:range rdf:resource="https://w3id.org/polifonia/ontology/cometa/ontology_URI#DataAccessibility"/>
        <rdfs:comment xml:lang="en">Associates the availability of a dataset to the way it can be accessed</rdfs:comment>
        <rdfs:label xml:lang="en">has accessibility</rdfs:label>
    </owl:ObjectProperty>
    


    <!-- https://w3id.org/polifonia/ontology/cometa/hasAssignment -->

    <owl:ObjectProperty rdf:about="https://w3id.org/polifonia/ontology/cometa/hasAssignment">
        <rdfs:domain rdf:resource="https://w3id.org/polifonia/ontology/cometa/ontology_URI#DatasetSplit"/>
        <rdfs:range rdf:resource="https://w3id.org/polifonia/ontology/cometa/ontology_URI#DatasetRecord"/>
        <rdfs:comment xml:lang="en">Associates a dataset split to a dataset record</rdfs:comment>
        <rdfs:label xml:lang="en">has assignment</rdfs:label>
        <rdfs:seeAlso rdf:resource="https://w3id.org/polifonia/ontology/cometa/ontology_URI#containsRecord"/>
        <owl:deprecated xml:lang="en">Not needed, since a dataset split is still a dataset, hence this can use contains record</owl:deprecated>
    </owl:ObjectProperty>
    


    <!-- https://w3id.org/polifonia/ontology/cometa/hasAvailability -->

    <owl:ObjectProperty rdf:about="https://w3id.org/polifonia/ontology/cometa/hasAvailability">
        <rdfs:domain rdf:resource="https://w3id.org/polifonia/ontology/cometa/ontology_URI#Dataset"/>
        <rdfs:domain rdf:resource="https://w3id.org/polifonia/ontology/cometa/ontology_URI#DatasetContent"/>
        <rdfs:range rdf:resource="https://w3id.org/polifonia/ontology/cometa/ontology_URI#DataAvailability"/>
        <rdfs:comment xml:lang="en">Associates a dataset to information related to its availability and access</rdfs:comment>
        <rdfs:label xml:lang="en">has availability</rdfs:label>
    </owl:ObjectProperty>
    


    <!-- https://w3id.org/polifonia/ontology/cometa/hasContent -->

    <owl:ObjectProperty rdf:about="https://w3id.org/polifonia/ontology/cometa/hasContent">
        <rdfs:domain rdf:resource="https://w3id.org/polifonia/ontology/cometa/ontology_URI#Dataset"/>
        <rdfs:range rdf:resource="https://w3id.org/polifonia/ontology/cometa/ontology_URI#DatasetContent"/>
        <rdfs:comment xml:lang="en">Associates a dataset to its content</rdfs:comment>
        <rdfs:label xml:lang="en">has content</rdfs:label>
    </owl:ObjectProperty>
    


    <!-- https://w3id.org/polifonia/ontology/cometa/hasContentType -->

    <owl:ObjectProperty rdf:about="https://w3id.org/polifonia/ontology/cometa/hasContentType">
        <rdfs:domain rdf:resource="https://w3id.org/polifonia/ontology/cometa/ContentAnnotation"/>
        <rdfs:domain rdf:resource="https://w3id.org/polifonia/ontology/cometa/RawDataContent"/>
        <rdfs:range rdf:resource="https://w3id.org/polifonia/ontology/cometa/ContentType"/>
        <rdfs:comment xml:lang="en">Associates raw data content or annotations to their type (e.g. tag, pattern, emotion).</rdfs:comment>
        <rdfs:label xml:lang="en">has content type</rdfs:label>
    </owl:ObjectProperty>
    


    <!-- https://w3id.org/polifonia/ontology/cometa/hasFeatureType -->

    <owl:ObjectProperty rdf:about="https://w3id.org/polifonia/ontology/cometa/hasFeatureType">
        <rdfs:domain rdf:resource="https://w3id.org/polifonia/ontology/cometa/ContentDescriptor"/>
        <rdfs:range rdf:resource="https://w3id.org/polifonia/ontology/cometa/ontology_URI#FeatureType"/>
        <rdfs:comment xml:lang="en">Associates a data descriptor to the type of feature it provides</rdfs:comment>
        <rdfs:label xml:lang="en">has feature type</rdfs:label>
    </owl:ObjectProperty>
    


    <!-- https://w3id.org/polifonia/ontology/cometa/hasModality -->

    <owl:ObjectProperty rdf:about="https://w3id.org/polifonia/ontology/cometa/hasModality">
        <rdfs:domain rdf:resource="https://w3id.org/polifonia/ontology/cometa/RawDataContent"/>
        <rdfs:range rdf:resource="https://w3id.org/polifonia/ontology/cometa/ontology_URI#DataModality"/>
        <rdfs:comment xml:lang="en">Associates raw data content to the modality the data provides</rdfs:comment>
        <rdfs:label xml:lang="en">has modality</rdfs:label>
    </owl:ObjectProperty>
    


    <!-- https://w3id.org/polifonia/ontology/cometa/hasSplit -->

    <owl:ObjectProperty rdf:about="https://w3id.org/polifonia/ontology/cometa/hasSplit">
        <rdfs:subPropertyOf rdf:resource="https://w3id.org/polifonia/ontology/cometa/hasSubset"/>
        <rdfs:domain rdf:resource="https://w3id.org/polifonia/ontology/cometa/ontology_URI#Dataset"/>
        <rdfs:range rdf:resource="https://w3id.org/polifonia/ontology/cometa/ontology_URI#Dataset"/>
        <rdfs:comment xml:lang="en">Associates a dataset to a proper partition (a particular subset) of it</rdfs:comment>
        <rdfs:label xml:lang="en">has split</rdfs:label>
    </owl:ObjectProperty>
    


    <!-- https://w3id.org/polifonia/ontology/cometa/hasSubset -->

    <owl:ObjectProperty rdf:about="https://w3id.org/polifonia/ontology/cometa/hasSubset">
        <rdfs:domain rdf:resource="https://w3id.org/polifonia/ontology/cometa/ontology_URI#Dataset"/>
        <rdfs:range rdf:resource="https://w3id.org/polifonia/ontology/cometa/ontology_URI#Dataset"/>
        <rdfs:comment xml:lang="en">A dataset can be a subset of another dataset</rdfs:comment>
        <rdfs:label xml:lang="en">has subset</rdfs:label>
    </owl:ObjectProperty>
    


    <!-- https://w3id.org/polifonia/ontology/cometa/includesContent -->

    <owl:ObjectProperty rdf:about="https://w3id.org/polifonia/ontology/cometa/includesContent">
        <rdfs:domain rdf:resource="https://w3id.org/polifonia/ontology/cometa/ontology_URI#DatasetRecord"/>
        <rdfs:range rdf:resource="https://w3id.org/polifonia/ontology/music-meta/MusicEntity"/>
        <rdfs:range rdf:resource="https://w3id.org/polifonia/ontology/music-meta/Recording"/>
        <rdfs:range rdf:resource="https://w3id.org/polifonia/ontology/music-meta/Release"/>
        <rdfs:range rdf:resource="https://w3id.org/polifonia/ontology/music-meta/Score"/>
        <rdfs:range rdf:resource="https://w3id.org/polifonia/ontology/music-meta/Text"/>
        <rdfs:comment xml:lang="en">Associates a dataset record to an atomic music element</rdfs:comment>
        <rdfs:label xml:lang="en">includes content</rdfs:label>
    </owl:ObjectProperty>
    


    <!-- https://w3id.org/polifonia/ontology/cometa/isAimedFor -->

    <owl:ObjectProperty rdf:about="https://w3id.org/polifonia/ontology/cometa/isAimedFor">
        <rdfs:domain rdf:resource="https://w3id.org/polifonia/ontology/cometa/ontology_URI#Dataset"/>
        <rdfs:range rdf:resource="https://w3id.org/polifonia/ontology/core/Task"/>
        <rdfs:comment xml:lang="en">Associates a dataset to a task it enables</rdfs:comment>
        <rdfs:label xml:lang="en">is aimed for</rdfs:label>
    </owl:ObjectProperty>
    


    <!-- https://w3id.org/polifonia/ontology/cometa/isMaintainedBy -->

    <owl:ObjectProperty rdf:about="https://w3id.org/polifonia/ontology/cometa/isMaintainedBy">
        <rdfs:domain rdf:resource="https://w3id.org/polifonia/ontology/cometa/ontology_URI#Dataset"/>
        <rdfs:range rdf:resource="https://w3id.org/polifonia/ontology/core/Agent"/>
        <rdfs:comment xml:lang="en">Associates a dataset to one of its maintainers (e.g. a person, an institution)</rdfs:comment>
        <rdfs:label xml:lang="en">is maintained by</rdfs:label>
    </owl:ObjectProperty>
    


    <!-- https://w3id.org/polifonia/ontology/cometa/ontology_URI#containsRecord -->

    <owl:ObjectProperty rdf:about="https://w3id.org/polifonia/ontology/cometa/ontology_URI#containsRecord">
        <rdfs:domain rdf:resource="https://w3id.org/polifonia/ontology/cometa/ontology_URI#Dataset"/>
        <rdfs:range rdf:resource="https://w3id.org/polifonia/ontology/cometa/ontology_URI#DatasetRecord"/>
        <rdfs:comment xml:lang="en">Associates a dataset record to the dataset it belongs to.</rdfs:comment>
        <rdfs:label xml:lang="en">contains record</rdfs:label>
    </owl:ObjectProperty>
    


    <!-- https://w3id.org/polifonia/ontology/music-meta/hasGenre -->

    <rdf:Description rdf:about="https://w3id.org/polifonia/ontology/music-meta/hasGenre">
        <rdfs:domain rdf:resource="https://w3id.org/polifonia/ontology/cometa/ontology_URI#Dataset"/>
        <rdfs:range rdf:resource="https://w3id.org/polifonia/ontology/music-meta/MusicGenre"/>
    </rdf:Description>
    


    <!-- https://w3id.org/polifonia/ontology/music-meta/hasLicense -->

    <rdf:Description rdf:about="https://w3id.org/polifonia/ontology/music-meta/hasLicense">
        <rdfs:domain rdf:resource="https://w3id.org/polifonia/ontology/cometa/ontology_URI#DataAvailability"/>
    </rdf:Description>
    


    <!-- 
    ///////////////////////////////////////////////////////////////////////////////////////
    //
    // Data properties
    //
    ///////////////////////////////////////////////////////////////////////////////////////
     -->

    


    <!-- https://w3id.org/polifonia/ontology/cometa/acronym -->

    <owl:DatatypeProperty rdf:about="https://w3id.org/polifonia/ontology/cometa/acronym">
        <rdfs:subPropertyOf rdf:resource="https://w3id.org/polifonia/ontology/core/name"/>
        <rdfs:range rdf:resource="http://www.w3.org/2001/XMLSchema#string"/>
    </owl:DatatypeProperty>
    


    <!-- https://w3id.org/polifonia/ontology/cometa/description -->

    <owl:DatatypeProperty rdf:about="https://w3id.org/polifonia/ontology/cometa/description">
        <rdfs:domain rdf:resource="http://www.w3.org/2002/07/owl#Thing"/>
        <rdfs:range rdf:resource="http://www.w3.org/2001/XMLSchema#string"/>
        <rdfs:comment xml:lang="en">A textual description</rdfs:comment>
        <rdfs:label xml:lang="en">description</rdfs:label>
    </owl:DatatypeProperty>
    


    <!-- https://w3id.org/polifonia/ontology/cometa/downloadLink -->

    <owl:DatatypeProperty rdf:about="https://w3id.org/polifonia/ontology/cometa/downloadLink">
        <rdfs:subPropertyOf rdf:resource="http://www.w3.org/2002/07/owl#topDataProperty"/>
        <rdfs:domain rdf:resource="https://w3id.org/polifonia/ontology/cometa/ontology_URI#DataAvailability"/>
        <rdfs:range rdf:resource="http://www.w3.org/2001/XMLSchema#anyURI"/>
        <rdfs:label xml:lang="en">download link</rdfs:label>
    </owl:DatatypeProperty>
    


    <!-- https://w3id.org/polifonia/ontology/cometa/recordCount -->

    <owl:DatatypeProperty rdf:about="https://w3id.org/polifonia/ontology/cometa/recordCount">
        <rdfs:domain rdf:resource="https://w3id.org/polifonia/ontology/cometa/ontology_URI#Dataset"/>
        <rdfs:domain rdf:resource="https://w3id.org/polifonia/ontology/cometa/ontology_URI#DatasetContent"/>
        <rdfs:range rdf:resource="http://www.w3.org/2001/XMLSchema#integer"/>
        <rdfs:comment xml:lang="en">The number of records that are contained in a data container</rdfs:comment>
        <rdfs:label>record count</rdfs:label>
    </owl:DatatypeProperty>
    


    <!-- https://w3id.org/polifonia/ontology/cometa/releaseDate -->

    <owl:DatatypeProperty rdf:about="https://w3id.org/polifonia/ontology/cometa/releaseDate">
        <rdfs:domain rdf:resource="http://www.w3.org/2002/07/owl#Thing"/>
        <rdfs:range rdf:resource="http://www.w3.org/2001/XMLSchema#dateTime"/>
        <rdfs:label xml:lang="en">release date</rdfs:label>
    </owl:DatatypeProperty>
    


    <!-- 
    ///////////////////////////////////////////////////////////////////////////////////////
    //
    // Classes
    //
    ///////////////////////////////////////////////////////////////////////////////////////
     -->

    


    <!-- https://w3id.org/polifonia/ontology/cometa/ContentAnnotation -->

    <owl:Class rdf:about="https://w3id.org/polifonia/ontology/cometa/ContentAnnotation">
        <rdfs:subClassOf rdf:resource="https://w3id.org/polifonia/ontology/cometa/ontology_URI#DatasetContent"/>
        <rdfs:comment xml:lang="en">Dataset content providing annotations that were produced or obtained from raw data content, or alternatively, from a data descriptor.</rdfs:comment>
        <rdfs:label xml:lang="en">Content Annotation</rdfs:label>
    </owl:Class>
    


    <!-- https://w3id.org/polifonia/ontology/cometa/ContentDescriptor -->

    <owl:Class rdf:about="https://w3id.org/polifonia/ontology/cometa/ContentDescriptor">
        <rdfs:subClassOf rdf:resource="https://w3id.org/polifonia/ontology/cometa/ontology_URI#DatasetContent"/>
        <rdfs:comment xml:lang="en">Dataset content that describes the raw data content via features or encodings extracted from the former. This should not be confused with an annotation, but as a supplementary view of the raw data content of a dataset.</rdfs:comment>
        <rdfs:label xml:lang="en">Content Descriptor</rdfs:label>
    </owl:Class>
    


    <!-- https://w3id.org/polifonia/ontology/cometa/ContentType -->

    <owl:Class rdf:about="https://w3id.org/polifonia/ontology/cometa/ContentType">
        <rdfs:comment xml:lang="en">Describes the type of content that the raw data, or its annotaitons, provide. In the music domain, this may correspond to chord, pattern, emotion, etc.</rdfs:comment>
        <rdfs:label xml:lang="en">Content Type</rdfs:label>
    </owl:Class>
    


    <!-- https://w3id.org/polifonia/ontology/cometa/RawDataContent -->

    <owl:Class rdf:about="https://w3id.org/polifonia/ontology/cometa/RawDataContent">
        <rdfs:subClassOf rdf:resource="https://w3id.org/polifonia/ontology/cometa/ontology_URI#DatasetContent"/>
        <rdfs:comment xml:lang="en">Dataset content providing raw data of structured (e.g. tabular data) or unstructured (e.g. audio files). For example, a dataset folder containing images can be described as raw data content.</rdfs:comment>
        <rdfs:label xml:lang="en">Raw Data Content</rdfs:label>
    </owl:Class>
    


    <!-- https://w3id.org/polifonia/ontology/cometa/ontology_URI#API -->

    <owl:Class rdf:about="https://w3id.org/polifonia/ontology/cometa/ontology_URI#API">
        <rdfs:comment xml:lang="en">Describes an Application Program Interface (API) for accessing, recreating, or extracting a dataset.</rdfs:comment>
        <rdfs:label xml:lang="en">API</rdfs:label>
        <rdfs:seeAlso rdf:resource="https://schema.org/APIReference"/>
        <rdfs:seeAlso rdf:resource="https://schema.org/WebAPI"/>
    </owl:Class>
    


    <!-- https://w3id.org/polifonia/ontology/cometa/ontology_URI#ContentAvailability -->

    <owl:Class rdf:about="https://w3id.org/polifonia/ontology/cometa/ontology_URI#ContentAvailability">
        <rdfs:comment xml:lang="en">Describes the availability of data content according to the release strategy and policies of the dataset. For example, a music dataset may provide complete data records (full tracks) or contain audio clips or snippets (excertps) only.</rdfs:comment>
        <rdfs:label xml:lang="en">Content Availability</rdfs:label>
    </owl:Class>
    


    <!-- https://w3id.org/polifonia/ontology/cometa/ontology_URI#DataAccessibility -->

    <owl:Class rdf:about="https://w3id.org/polifonia/ontology/cometa/ontology_URI#DataAccessibility">
        <rdfs:comment xml:lang="en">Describes the accessibility of a dataset, instructing users on the modalities put in the place by the maintaners to access its content.</rdfs:comment>
        <rdfs:label xml:lang="en">Data Accessibility</rdfs:label>
    </owl:Class>
    


    <!-- https://w3id.org/polifonia/ontology/cometa/ontology_URI#DataAvailability -->

    <owl:Class rdf:about="https://w3id.org/polifonia/ontology/cometa/ontology_URI#DataAvailability">
        <rdfs:comment xml:lang="en">Describes the available of a dataset as a whole, or of a part of its content.</rdfs:comment>
        <rdfs:label xml:lang="en">Data Availability</rdfs:label>
    </owl:Class>
    


    <!-- https://w3id.org/polifonia/ontology/cometa/ontology_URI#DataFormat -->

    <owl:Class rdf:about="https://w3id.org/polifonia/ontology/cometa/ontology_URI#DataFormat">
        <rdfs:comment xml:lang="en">The format of the data in which content is provided.</rdfs:comment>
        <rdfs:label xml:lang="en">Data Format</rdfs:label>
    </owl:Class>
    


    <!-- https://w3id.org/polifonia/ontology/cometa/ontology_URI#DataModality -->

    <owl:Class rdf:about="https://w3id.org/polifonia/ontology/cometa/ontology_URI#DataModality">
        <rdfs:comment xml:lang="en">Describes the modality of dataset content such as audio, video, image, etc.</rdfs:comment>
        <rdfs:label xml:lang="en">Data Modality</rdfs:label>
    </owl:Class>
    


    <!-- https://w3id.org/polifonia/ontology/cometa/ontology_URI#Dataset -->

    <owl:Class rdf:about="https://w3id.org/polifonia/ontology/cometa/ontology_URI#Dataset">
        <rdfs:subClassOf rdf:resource="https://w3id.org/polifonia/ontology/music-meta/Collection"/>
        <rdfs:comment xml:lang="en">A container of data records with summative properties that allow the contextualisation of its content, availability and licensing.</rdfs:comment>
        <rdfs:label xml:lang="en">Dataset</rdfs:label>
    </owl:Class>
    


    <!-- https://w3id.org/polifonia/ontology/cometa/ontology_URI#DatasetContent -->

    <owl:Class rdf:about="https://w3id.org/polifonia/ontology/cometa/ontology_URI#DatasetContent">
        <rdfs:comment xml:lang="en">Describe the content of a dataset from a summative perspective (e.g. the audio content of a music collection, the audio features it provides, etc.) and its production process (provenance).</rdfs:comment>
        <rdfs:label xml:lang="en">Dataset Content</rdfs:label>
    </owl:Class>
    


    <!-- https://w3id.org/polifonia/ontology/cometa/ontology_URI#DatasetRecord -->

    <owl:Class rdf:about="https://w3id.org/polifonia/ontology/cometa/ontology_URI#DatasetRecord">
        <rdfs:comment xml:lang="en">A record of a dataset, providing references to its properties and annotations.</rdfs:comment>
        <rdfs:label xml:lang="en">Dataset Record</rdfs:label>
    </owl:Class>
    


    <!-- https://w3id.org/polifonia/ontology/cometa/ontology_URI#DatasetSplit -->

    <owl:Class rdf:about="https://w3id.org/polifonia/ontology/cometa/ontology_URI#DatasetSplit">
        <rdfs:subClassOf rdf:resource="https://w3id.org/polifonia/ontology/cometa/ontology_URI#Dataset"/>
        <rdfs:comment xml:lang="en">Describes a partition of a dataset via its association with individual data record, which can be used for training, validating, or testing a computational method.</rdfs:comment>
        <rdfs:label xml:lang="en">Dataset Split</rdfs:label>
    </owl:Class>
    


    <!-- https://w3id.org/polifonia/ontology/cometa/ontology_URI#FeatureType -->

    <owl:Class rdf:about="https://w3id.org/polifonia/ontology/cometa/ontology_URI#FeatureType">
        <rdfs:comment xml:lang="en">Describes the type of feature provided by a content descriptor.</rdfs:comment>
        <rdfs:label xml:lang="en">Feature Type</rdfs:label>
    </owl:Class>
    


    <!-- https://w3id.org/polifonia/ontology/cometa/ontology_URI#ProductionMethod -->

    <owl:Class rdf:about="https://w3id.org/polifonia/ontology/cometa/ontology_URI#ProductionMethod">
        <rdfs:comment xml:lang="en">A production method is an activity that generates one or more artefacts that joinlty characterises data content.</rdfs:comment>
        <rdfs:label xml:lang="en">Production Method</rdfs:label>
    </owl:Class>
    


    <!-- https://w3id.org/polifonia/ontology/cometa/ontology_URI#SplitType -->

    <owl:Class rdf:about="https://w3id.org/polifonia/ontology/cometa/ontology_URI#SplitType">
        <rdfs:comment xml:lang="en">The type of a split that associates a function to the corresponding data partitions (e.g. a training set).</rdfs:comment>
        <rdfs:label xml:lang="en">Split Type</rdfs:label>
    </owl:Class>
    


    <!-- 
    ///////////////////////////////////////////////////////////////////////////////////////
    //
    // Individuals
    //
    ///////////////////////////////////////////////////////////////////////////////////////
     -->

    


    <!-- https://w3id.org/polifonia/ontology/cometa/ABC -->

    <owl:NamedIndividual rdf:about="https://w3id.org/polifonia/ontology/cometa/ABC">
        <rdf:type rdf:resource="https://w3id.org/polifonia/ontology/cometa/ontology_URI#DataFormat"/>
    </owl:NamedIndividual>
    


    <!-- https://w3id.org/polifonia/ontology/cometa/Audio -->

    <owl:NamedIndividual rdf:about="https://w3id.org/polifonia/ontology/cometa/Audio">
        <rdf:type rdf:resource="https://w3id.org/polifonia/ontology/cometa/ontology_URI#DataModality"/>
        <rdfs:comment xml:lang="en">Audio as a modality</rdfs:comment>
        <rdfs:label xml:lang="en">Audio</rdfs:label>
    </owl:NamedIndividual>
    


    <!-- https://w3id.org/polifonia/ontology/cometa/CSV -->

    <owl:NamedIndividual rdf:about="https://w3id.org/polifonia/ontology/cometa/CSV">
        <rdf:type rdf:resource="https://w3id.org/polifonia/ontology/cometa/ontology_URI#DataFormat"/>
    </owl:NamedIndividual>
    


    <!-- https://w3id.org/polifonia/ontology/cometa/Chord -->

    <owl:NamedIndividual rdf:about="https://w3id.org/polifonia/ontology/cometa/Chord">
        <rdf:type rdf:resource="https://w3id.org/polifonia/ontology/cometa/ContentType"/>
        <rdfs:comment xml:lang="en">Chords refer to harmonic structures found in music data.</rdfs:comment>
        <rdfs:label xml:lang="en">Chord</rdfs:label>
    </owl:NamedIndividual>
    


    <!-- https://w3id.org/polifonia/ontology/cometa/ChromaFeatures -->

    <owl:NamedIndividual rdf:about="https://w3id.org/polifonia/ontology/cometa/ChromaFeatures">
        <rdf:type rdf:resource="https://w3id.org/polifonia/ontology/cometa/ontology_URI#FeatureType"/>
        <rdfs:comment xml:lang="en">Chroma-based features are descriptor of pitched audio signals (e.g. music).</rdfs:comment>
        <rdfs:label xml:lang="en">Chroma Features</rdfs:label>
    </owl:NamedIndividual>
    


    <!-- https://w3id.org/polifonia/ontology/cometa/Computational -->

    <owl:NamedIndividual rdf:about="https://w3id.org/polifonia/ontology/cometa/Computational">
        <rdf:type rdf:resource="https://w3id.org/polifonia/ontology/cometa/ontology_URI#ProductionMethod"/>
        <rdfs:comment xml:lang="en">A production method based on a computational procedure</rdfs:comment>
        <rdfs:label xml:lang="en">Algorithmic</rdfs:label>
        <rdfs:label xml:lang="en">Computational</rdfs:label>
    </owl:NamedIndividual>
    


    <!-- https://w3id.org/polifonia/ontology/cometa/Crowdsourced -->

    <owl:NamedIndividual rdf:about="https://w3id.org/polifonia/ontology/cometa/Crowdsourced">
        <rdf:type rdf:resource="https://w3id.org/polifonia/ontology/cometa/ontology_URI#ProductionMethod"/>
        <rdfs:comment xml:lang="en">A production method collecting data via crowdsourcing</rdfs:comment>
        <rdfs:label xml:lang="en">Crowdsourced</rdfs:label>
    </owl:NamedIndividual>
    


    <!-- https://w3id.org/polifonia/ontology/cometa/DevelopmentSet -->

    <owl:NamedIndividual rdf:about="https://w3id.org/polifonia/ontology/cometa/DevelopmentSet">
        <rdf:type rdf:resource="https://w3id.org/polifonia/ontology/cometa/ontology_URI#SplitType"/>
        <rdfs:comment xml:lang="en">A dataset split including the validation and test sets</rdfs:comment>
        <rdfs:label xml:lang="en">Development Set</rdfs:label>
    </owl:NamedIndividual>
    


    <!-- https://w3id.org/polifonia/ontology/cometa/Emotion -->

    <owl:NamedIndividual rdf:about="https://w3id.org/polifonia/ontology/cometa/Emotion">
        <rdf:type rdf:resource="https://w3id.org/polifonia/ontology/cometa/ContentType"/>
        <rdfs:comment xml:lang="en">Emotion can be either perceived or induced from the data</rdfs:comment>
        <rdfs:label xml:lang="en">Emotion</rdfs:label>
    </owl:NamedIndividual>
    


    <!-- https://w3id.org/polifonia/ontology/cometa/ExpertHuman -->

    <owl:NamedIndividual rdf:about="https://w3id.org/polifonia/ontology/cometa/ExpertHuman">
        <rdf:type rdf:resource="https://w3id.org/polifonia/ontology/cometa/ontology_URI#ProductionMethod"/>
        <rdfs:comment xml:lang="en">A production method relying on human analysis</rdfs:comment>
        <rdfs:comment xml:lang="en">Expert Human</rdfs:comment>
    </owl:NamedIndividual>
    


    <!-- https://w3id.org/polifonia/ontology/cometa/FLAC -->

    <owl:NamedIndividual rdf:about="https://w3id.org/polifonia/ontology/cometa/FLAC">
        <rdf:type rdf:resource="https://w3id.org/polifonia/ontology/cometa/ontology_URI#DataFormat"/>
    </owl:NamedIndividual>
    


    <!-- https://w3id.org/polifonia/ontology/cometa/FullContent -->

    <owl:NamedIndividual rdf:about="https://w3id.org/polifonia/ontology/cometa/FullContent">
        <rdf:type rdf:resource="https://w3id.org/polifonia/ontology/cometa/ontology_URI#ContentAvailability"/>
        <rdfs:comment xml:lang="en">Data is made available in its entirety (e.g. full audio tracks)</rdfs:comment>
        <rdfs:label xml:lang="en">Full Content</rdfs:label>
    </owl:NamedIndividual>
    


    <!-- https://w3id.org/polifonia/ontology/cometa/Image -->

    <owl:NamedIndividual rdf:about="https://w3id.org/polifonia/ontology/cometa/Image">
        <rdf:type rdf:resource="https://w3id.org/polifonia/ontology/cometa/ontology_URI#DataModality"/>
        <rdfs:comment xml:lang="en">Image as a modality</rdfs:comment>
        <rdfs:label xml:lang="en">Image</rdfs:label>
    </owl:NamedIndividual>
    


    <!-- https://w3id.org/polifonia/ontology/cometa/JAMS -->

    <owl:NamedIndividual rdf:about="https://w3id.org/polifonia/ontology/cometa/JAMS">
        <rdf:type rdf:resource="https://w3id.org/polifonia/ontology/cometa/ontology_URI#DataFormat"/>
    </owl:NamedIndividual>
    


    <!-- https://w3id.org/polifonia/ontology/cometa/JSON -->

    <owl:NamedIndividual rdf:about="https://w3id.org/polifonia/ontology/cometa/JSON">
        <rdf:type rdf:resource="https://w3id.org/polifonia/ontology/cometa/ontology_URI#DataFormat"/>
    </owl:NamedIndividual>
    


    <!-- https://w3id.org/polifonia/ontology/cometa/Kern -->

    <owl:NamedIndividual rdf:about="https://w3id.org/polifonia/ontology/cometa/Kern">
        <rdf:type rdf:resource="https://w3id.org/polifonia/ontology/cometa/ontology_URI#DataFormat"/>
    </owl:NamedIndividual>
    


    <!-- https://w3id.org/polifonia/ontology/cometa/MEI -->

    <owl:NamedIndividual rdf:about="https://w3id.org/polifonia/ontology/cometa/MEI">
        <rdf:type rdf:resource="https://w3id.org/polifonia/ontology/cometa/ontology_URI#DataFormat"/>
    </owl:NamedIndividual>
    


    <!-- https://w3id.org/polifonia/ontology/cometa/MELSpectogram -->

    <owl:NamedIndividual rdf:about="https://w3id.org/polifonia/ontology/cometa/MELSpectogram">
        <rdf:type rdf:resource="https://w3id.org/polifonia/ontology/cometa/ontology_URI#FeatureType"/>
        <rdfs:comment xml:lang="en">A Mel Spectrogram is a descriptor, or feature, of an audio signal.</rdfs:comment>
        <rdfs:label xml:lang="en">Mel Spectogram</rdfs:label>
    </owl:NamedIndividual>
    


    <!-- https://w3id.org/polifonia/ontology/cometa/MFCCFeatures -->

    <owl:NamedIndividual rdf:about="https://w3id.org/polifonia/ontology/cometa/MFCCFeatures">
        <rdf:type rdf:resource="https://w3id.org/polifonia/ontology/cometa/ontology_URI#FeatureType"/>
        <rdfs:comment xml:lang="en">MFCC Features</rdfs:comment>
        <rdfs:comment xml:lang="en">Mel-frequency cepstral coefficients (MFCCs) are an audio features.</rdfs:comment>
    </owl:NamedIndividual>
    


    <!-- https://w3id.org/polifonia/ontology/cometa/MIDI -->

    <owl:NamedIndividual rdf:about="https://w3id.org/polifonia/ontology/cometa/MIDI">
        <rdf:type rdf:resource="https://w3id.org/polifonia/ontology/cometa/ontology_URI#DataFormat"/>
    </owl:NamedIndividual>
    


    <!-- https://w3id.org/polifonia/ontology/cometa/MP3 -->

    <owl:NamedIndividual rdf:about="https://w3id.org/polifonia/ontology/cometa/MP3">
        <rdf:type rdf:resource="https://w3id.org/polifonia/ontology/cometa/ontology_URI#DataFormat"/>
    </owl:NamedIndividual>
    


    <!-- https://w3id.org/polifonia/ontology/cometa/MusicXML -->

    <owl:NamedIndividual rdf:about="https://w3id.org/polifonia/ontology/cometa/MusicXML">
        <rdf:type rdf:resource="https://w3id.org/polifonia/ontology/cometa/ontology_URI#DataFormat"/>
    </owl:NamedIndividual>
    


    <!-- https://w3id.org/polifonia/ontology/cometa/OnRequestAccess -->

    <owl:NamedIndividual rdf:about="https://w3id.org/polifonia/ontology/cometa/OnRequestAccess">
        <rdf:type rdf:resource="https://w3id.org/polifonia/ontology/cometa/ontology_URI#DataAccessibility"/>
        <rdfs:comment xml:lang="en">Access to the dataset undergoes a request procedure</rdfs:comment>
        <rdfs:label xml:lang="en">On Request Access</rdfs:label>
    </owl:NamedIndividual>
    


    <!-- https://w3id.org/polifonia/ontology/cometa/OpenAccess -->

    <owl:NamedIndividual rdf:about="https://w3id.org/polifonia/ontology/cometa/OpenAccess">
        <rdf:type rdf:resource="https://w3id.org/polifonia/ontology/cometa/ontology_URI#DataAccessibility"/>
        <rdfs:comment xml:lang="en">Access to the dataset is open</rdfs:comment>
        <rdfs:label xml:lang="en">Open Access</rdfs:label>
    </owl:NamedIndividual>
    


    <!-- https://w3id.org/polifonia/ontology/cometa/Pattern -->

    <owl:NamedIndividual rdf:about="https://w3id.org/polifonia/ontology/cometa/Pattern">
        <rdf:type rdf:resource="https://w3id.org/polifonia/ontology/cometa/ContentType"/>
        <rdfs:comment xml:lang="en">Patterns are usually found in the data to express and formalise regularities.</rdfs:comment>
        <rdfs:label xml:lang="en">Pattern</rdfs:label>
    </owl:NamedIndividual>
    


    <!-- https://w3id.org/polifonia/ontology/cometa/PreviewContent -->

    <owl:NamedIndividual rdf:about="https://w3id.org/polifonia/ontology/cometa/PreviewContent">
        <rdf:type rdf:resource="https://w3id.org/polifonia/ontology/cometa/ontology_URI#ContentAvailability"/>
        <rdfs:comment xml:lang="en">Data is made available in partial form (e.g. audio snippets).</rdfs:comment>
        <rdfs:label xml:lang="en">Preview Content</rdfs:label>
    </owl:NamedIndividual>
    


    <!-- https://w3id.org/polifonia/ontology/cometa/Structure -->

    <owl:NamedIndividual rdf:about="https://w3id.org/polifonia/ontology/cometa/Structure">
        <rdf:type rdf:resource="https://w3id.org/polifonia/ontology/cometa/ContentType"/>
        <rdfs:comment xml:lang="en">Structural content refers to segments or sub-sequencies found in sequential data. In the context of music, this may correspond to segments related to musical form (e.g. motifs, phrases, sections).</rdfs:comment>
        <rdfs:label xml:lang="en">Structure</rdfs:label>
    </owl:NamedIndividual>
    


    <!-- https://w3id.org/polifonia/ontology/cometa/TestSet -->

    <owl:NamedIndividual rdf:about="https://w3id.org/polifonia/ontology/cometa/TestSet">
        <rdf:type rdf:resource="https://w3id.org/polifonia/ontology/cometa/ontology_URI#SplitType"/>
        <rdfs:comment xml:lang="en">A split including test data</rdfs:comment>
        <rdfs:label xml:lang="en">Test Set</rdfs:label>
    </owl:NamedIndividual>
    


    <!-- https://w3id.org/polifonia/ontology/cometa/Text -->

    <owl:NamedIndividual rdf:about="https://w3id.org/polifonia/ontology/cometa/Text">
        <rdf:type rdf:resource="https://w3id.org/polifonia/ontology/cometa/ontology_URI#DataModality"/>
        <rdfs:comment xml:lang="en">Text as a modality</rdfs:comment>
        <rdfs:label xml:lang="en">Text</rdfs:label>
    </owl:NamedIndividual>
    


    <!-- https://w3id.org/polifonia/ontology/cometa/TrainingSet -->

    <owl:NamedIndividual rdf:about="https://w3id.org/polifonia/ontology/cometa/TrainingSet">
        <rdf:type rdf:resource="https://w3id.org/polifonia/ontology/cometa/ontology_URI#SplitType"/>
        <rdfs:comment xml:lang="en">A split including training data</rdfs:comment>
        <rdfs:label xml:lang="en">Training Set</rdfs:label>
    </owl:NamedIndividual>
    


    <!-- https://w3id.org/polifonia/ontology/cometa/ValidationSet -->

    <owl:NamedIndividual rdf:about="https://w3id.org/polifonia/ontology/cometa/ValidationSet">
        <rdf:type rdf:resource="https://w3id.org/polifonia/ontology/cometa/ontology_URI#SplitType"/>
        <rdfs:comment xml:lang="en">A split including validation data</rdfs:comment>
        <rdfs:label xml:lang="en">Validation Set</rdfs:label>
    </owl:NamedIndividual>
    


    <!-- https://w3id.org/polifonia/ontology/cometa/Video -->

    <owl:NamedIndividual rdf:about="https://w3id.org/polifonia/ontology/cometa/Video">
        <rdf:type rdf:resource="https://w3id.org/polifonia/ontology/cometa/ontology_URI#DataModality"/>
        <rdfs:comment xml:lang="en">Video as a modality</rdfs:comment>
        <rdfs:label xml:lang="en">Video</rdfs:label>
    </owl:NamedIndividual>
    


    <!-- https://w3id.org/polifonia/ontology/cometa/WAV -->

    <owl:NamedIndividual rdf:about="https://w3id.org/polifonia/ontology/cometa/WAV">
        <rdf:type rdf:resource="https://w3id.org/polifonia/ontology/cometa/ontology_URI#DataFormat"/>
    </owl:NamedIndividual>
</rdf:RDF>



<!-- Generated by the OWL API (version 4.5.9.2019-02-01T07:24:44Z) https://github.com/owlcs/owlapi -->

